theories/UntypedAlgorithmicConversion.v
@@ -1,4 +1,11 @@
 (** * LogRel.UntypedAlgorithmicConversion: alternative definition of algorithmic conversion. *)
+
+From LogRel Require Import PremisePreserve.
+From MetaCoq.Utils Require Import bytestring.
+From MetaCoq.Template Require Import Loader.
+
+Open Scope bs.
+
 From LogRel.AutoSubst Require Import core unscoped Ast Extra.
 From LogRel Require Import Utils BasicAst Notations Context NormalForms Weakening
   UntypedReduction GenericTyping DeclarativeTyping DeclarativeInstance
@@ -572,7 +579,7 @@ Section NeutralConversion.
     eassumption.
   Qed.
 
-  Lemma conv_ne_complete_pos (Γ : context) (A A' m n : term) :
+  (* Lemma conv_ne_complete_pos (Γ : context) (A A' m n : term) :
     [A ⤳* A'] ->
     isPosType A' ->
     whne m ->
@@ -667,9 +674,93 @@ Section NeutralConversion.
     eapply conv_ne_complete_pos ; tea.
     1: now eapply red.
     now constructor.
-  Qed.
+  Qed. *)
 
 End NeutralConversion.
+
+Section Invariants.
+
+  Unset MetaCoq Strict Unquote Universe Mode.
+
+  MetaCoq Quote Definition conv_precond :=
+  (fun u v => ∑ (Γ : context) A, [Γ |-[de] u : A] × [Γ |-[de] v : A]).
+  MetaCoq Quote Definition convred_precond :=
+  (fun u v => ∑ (Γ : context) A, [Γ |-[de] u : A] × [Γ |-[de] v : A]).
+  MetaCoq Quote Definition convneu_precond :=
+  (fun u v => ∑ (Γ : context), well_typed (ta := de) Γ u × well_typed (ta := de) Γ v).
+
+  #[local] Definition pre_cond (hyp : Ast.term) : Ast.term :=
+  match hyp with
+    | Ast.tApp c (u :: v :: nil)%list =>
+        if (c ?= <% UConvAlg %>) then Ast.tApp conv_precond (u :: v :: nil)%list
+        else if (c ?= <% UConvRedAlg %>) then Ast.tApp convred_precond (u :: v :: nil)%list
+        else if (c ?= <% UConvNeuAlg %>) then Ast.tApp convneu_precond (u :: v :: nil)%list
+        else hyp
+    | _ => hyp
+  end.
+
+  MetaCoq Quote Definition conv_postcond :=
+  (fun t u =>
+    (forall Γ, [Γ |-[de] t] -> [Γ |-[de] u] -> [Γ |-[al] t ≅ u]) ×
+    (forall Γ A, [Γ |-[de] t : A] -> [Γ |-[de] u : A] -> [Γ |-[al] t ≅ u : A])).
+
+  MetaCoq Quote Definition convred_postcond :=
+  (fun t u => 
+    (forall Γ, [Γ |-[de] t] -> [Γ |-[de] u] -> [Γ |-[al] t ≅h u]) ×
+    (forall Γ A, isType A -> [Γ |-[de] t : A] -> [Γ |-[de] u : A] -> [Γ |-[al] t ≅h u : A])).
+  
+  MetaCoq Quote Definition convneu_postcond :=
+  (fun t u => 
+    forall Γ A A', [Γ |-[de] t : A] -> [Γ |-[de] u : A'] ->
+    ∑ A'', [× [Γ |-[al] t ~ u ▹ A''], [Γ |-[de] A'' ≅ A] & [Γ |-[de] A'' ≅ A']]).
+
+  #[local] Definition post_cond (hyp : Ast.term) : Ast.term :=
+  match hyp with
+    | Ast.tApp c (u :: v :: nil)%list =>
+        if (c ?= <% UConvAlg %>) then Ast.tApp conv_postcond (u :: v :: nil)%list
+        else if (c ?= <% UConvRedAlg %>) then Ast.tApp convred_postcond (u :: v :: nil)%list
+        else if (c ?= <% UConvNeuAlg %>) then Ast.tApp convneu_postcond (u :: v :: nil)%list
+        else hyp
+    | _ => hyp
+  end.
+
+Lemma termConvRed_concl : $run (constructor_concl_preserve pre_cond post_cond "termConvRed").
+Proof.
+  intros * Ht Hu [Hty Htm].
+  split.
+  + intros.
+    econstructor ; eauto.
+    eapply Hty.
+    all: now eapply subject_reduction_raw_ty.
+  + intros.
+    assert [Γ |-[de] A] as [? red]%type_normalisation by boundary.
+    eapply subject_reduction_type in red as [] ; refold.
+    2: boundary.
+    econstructor ; eauto.
+    eapply Htm.
+    * eapply type_isType ; tea.
+      boundary.
+    * eapply subject_reduction_raw ; tea.
+      gen_typing.
+    * eapply subject_reduction_raw ; tea.
+      gen_typing.
+Qed.
+
+
+
+
+(* Proof.
+  intros m n t u [Γ [[? (?&(?&?&[-> ])&?)%termGen'] [? (?&(?&?&[-> ])&?)%termGen']]].
+  exists Γ.
+  split ; now eexists.
+Qed. *)
+
+Lemma bar : $run (constructor_premise_preserve pre_cond post_cond 1 "NeLamUAlg").
+Proof.
+intros * ? (Γ&A&[? (?&[? [->]]&?)%termGen']).
+do 2 eexists ; split ; tea.
+eapply (typing_wk (ρ := wk1 _ _)).
+1: eapply t0
 
 Section Soundness.
 
@@ -689,6 +780,7 @@ Section Soundness.
     UAlgoConvInductionConcl PEq PRedEq PNeEq.
   Proof.
     subst PEq PRedEq PNeEq.
+    unfold UAlgoConvInductionConcl.
     apply UAlgoConvInduction.
     - intros * Ht Hu Ht' [Hty Htm].
       split.
